@@ -92,4 +92,5 @@ import MachCSL.WpDevDmaStep
 import MachCSL.WpDmaCtx
 import MachCSL.WireInv
 import MachCSL.WpWire
+import MachCSL.WpDevDmaStepV
 import MachCSL.WpSmodeTime
